examples/Lambda.lean
@@ -48,7 +48,8 @@ inductive Term where
   GParser.ws *> GParser.capture (GParser.takeWhile1 Ascii.isAlpha)
 
 /-- Parse one lambda term. -/
-def term : GParser conditional Term :=
+def term
+    : GParser conditional Term :=
   GParser.fix fun term =>
     let var : GParser conditional Term :=
       Term.var <$> GParser.capture (GParser.takeWhile1 Ascii.isAlpha)
